DeBruijnSSA/BinSyntax/Rewrite/Term/Induction.lean
@@ -1,0 +1,12 @@
+import DeBruijnSSA.BinSyntax.Rewrite.Term.Setoid
+
+import Discretion.Utils.Quotient
+
+namespace BinSyntax
+
+variable [Φ: EffInstSet φ (Ty α) ε] [PartialOrder α] [SemilatticeSup ε] [OrderBot ε]
+
+namespace Term
+
+
+-- ...
